memory_refinements/memory_map_refine.v
@@ -1,5 +1,6 @@
 (* Copyright (c) 2012-2015, Robbert Krebbers. *)
 (* This file is distributed under the terms of the BSD license. *)
+From stdpp Require Import fin_maps.
 Require Export memory_map memory_trees_refine.
 Local Open Scope ctype_scope.
 
